fixed brackets and identation

SSA/Projects/RISCV64/Semantics.lean
@@ -1,5 +1,8 @@
 import SSA.Core.MLIRSyntax.EDSL
+import SSA.Projects.InstCombine.ForLean
 set_option maxHeartbeats 1000000000000000000
+
+open BitVec
 /-!
   ## Dialect semantics
   This file contains the semantics for each modelled `RISCV-64` dialect instruction
@@ -10,6 +13,10 @@ set_option maxHeartbeats 1000000000000000000
   we rewrote the Sail semantics into pure bit vector only operations including a proof
   of correctness.
   This rewrite should allow to gain in automation using the bv_decide.
+
+  The instruction semantics suffixed by "bv" indicates that it is
+  the purely bit vector defintion where we removed
+  toInt/toNat calls.
 -/
 
 namespace RV64Semantics
@@ -25,22 +32,86 @@ def UTYPE_pure64_AUIPC (imm : BitVec 20) (pc : BitVec 64) : BitVec 64 :=
   BitVec.add (BitVec.signExtend 64 (BitVec.append imm (0x000 : BitVec 12))) pc
 
 def SHIFTIWOP_pure64_RISCV_SLLIW (shamt : BitVec 5) (rs1_val : BitVec 64) : BitVec 64 :=
-  BitVec.signExtend 64 ((BitVec.extractLsb' 0 32 rs1_val) <<< shamt)
+    BitVec.signExtend 64 (BitVec.shiftLeft (BitVec.extractLsb' 0 32 rs1_val) (shamt).toNat)
+
+def SHIFTIWOP_pure64_RISCV_SLLIW_bv (shamt : BitVec 5) (rs1_val : BitVec 64) : BitVec 64 :=
+    BitVec.signExtend 64 ((BitVec.extractLsb' 0 32 rs1_val)  <<< shamt)
+
+theorem SHIFTIWOP_pure64_RISCV_SLLIW_eq_SHIFTIWOP_pure64_RISCV_SLLIW_bv (shamt : BitVec 5) (rs1_val : BitVec 64) :
+    SHIFTIWOP_pure64_RISCV_SLLIW shamt rs1_val = SHIFTIWOP_pure64_RISCV_SLLIW_bv shamt rs1_val :=
+  by
+  unfold SHIFTIWOP_pure64_RISCV_SLLIW SHIFTIWOP_pure64_RISCV_SLLIW_bv
+  rfl
 
 def SHIFTIWOP_pure64_RISCV_SRLIW (shamt : BitVec 5) (rs1_val : BitVec 64) : BitVec 64 :=
-  BitVec.signExtend 64 ((BitVec.extractLsb' 0 32 rs1_val) >>> shamt)
+    BitVec.signExtend 64 (BitVec.ushiftRight (BitVec.extractLsb' 0 32 rs1_val) (shamt).toNat)
+
+def SHIFTIWOP_pure64_RISCV_SRLIW_bv (shamt : BitVec 5) (rs1_val : BitVec 64) : BitVec 64 :=
+    BitVec.signExtend 64 ((BitVec.extractLsb' 0 32 rs1_val) >>> shamt)
+
+theorem  SHIFTIWOP_pure64_RISCV_SRLIW_eq_SHIFTIWOP_pure64_RISCV_SRLIW_bv (shamt : BitVec 5) (rs1_val : BitVec 64) :
+    SHIFTIWOP_pure64_RISCV_SRLIW shamt rs1_val =  SHIFTIWOP_pure64_RISCV_SRLIW_bv shamt rs1_val :=
+  by
+  unfold SHIFTIWOP_pure64_RISCV_SRLIW SHIFTIWOP_pure64_RISCV_SRLIW_bv
+  rfl
 
 def SHIFTIWOP_pure64_RISCV_SRAIW (shamt : BitVec 5) (rs1_val : BitVec 64) : BitVec 64 :=
-  BitVec.signExtend 64 (BitVec.sshiftRight' (BitVec.extractLsb 31 0 rs1_val) shamt)
+    BitVec.signExtend 64
+      (BitVec.setWidth 32
+       (BitVec.extractLsb
+         (31 + shamt.toNat)
+          shamt.toNat
+          (BitVec.signExtend (32 + shamt.toNat) (BitVec.extractLsb 31 0 rs1_val))))
+
+def SHIFTIWOP_pure64_RISCV_SRAIW_bv (shamt : BitVec 5) (rs1_val : BitVec 64) : BitVec 64 :=
+    BitVec.signExtend 64 (BitVec.sshiftRight' (BitVec.extractLsb 31 0 rs1_val) shamt)
+
+theorem SHIFTIWOP_pure64_RISCV_SRAIW_eq_SHIFTIWOP_pure64_RISCV_SRAIW_bv (shamt : BitVec 5) (rs1_val : BitVec 64) :
+    SHIFTIWOP_pure64_RISCV_SRAIW shamt rs1_val = SHIFTIWOP_pure64_RISCV_SRAIW_bv shamt rs1_val :=
+  by
+  unfold SHIFTIWOP_pure64_RISCV_SRAIW SHIFTIWOP_pure64_RISCV_SRAIW_bv
+  rw [← sshiftRight_eq_setWidth_extractLsb_signExtend]
+  rfl
 
 def SHIFTIOP_pure64_RISCV_SLLI (shamt : BitVec 6) (rs1_val : BitVec 64) : BitVec 64 :=
-  rs1_val <<< shamt
+    BitVec.shiftLeft rs1_val shamt.toNat
+
+def  SHIFTIOP_pure64_RISCV_SLLI_bv (shamt : BitVec 6) (rs1_val : BitVec 64) : BitVec 64 :=
+    rs1_val <<< shamt
+
+theorem SHIFTIOP_pure64_RISCV_SLLI_eq_SHIFTIOP_pure64_RISCV_SLLI_bv :
+    SHIFTIOP_pure64_RISCV_SLLI shamt rs1_val = SHIFTIOP_pure64_RISCV_SLLI_bv shamt rs1_val := by
+  unfold SHIFTIOP_pure64_RISCV_SLLI SHIFTIOP_pure64_RISCV_SLLI_bv
+  simp only [BitVec.shiftLeft_eq, BitVec.shiftLeft_eq']
+
 
 def SHIFTIOP_pure64_RISCV_SRLI (shamt : BitVec 6) (rs1_val : BitVec 64) : BitVec 64 :=
-  rs1_val >>> shamt
+    BitVec.ushiftRight rs1_val shamt.toNat
 
-def SHIFTIOP_pure64_RISCV_SRAI (shamt : BitVec 6) (rs1_val : BitVec 64) : BitVec 64 :=
-  BitVec.sshiftRight' rs1_val  shamt
+def SHIFTIOP_pure64_RISCV_SRLI_bv (shamt : BitVec 6) (rs1_val : BitVec 64) : BitVec 64 :=
+    rs1_val >>> shamt
+
+theorem SHIFTIOP_pure64_RISCV_SRLI_eq_SHIFTIOP_pure64_RISCV_SRLI_bv (shamt : BitVec 6) (rs1_val : BitVec 64) :
+    SHIFTIOP_pure64_RISCV_SRLI shamt rs1_val = SHIFTIOP_pure64_RISCV_SRLI_bv shamt rs1_val := by
+  unfold SHIFTIOP_pure64_RISCV_SRLI SHIFTIOP_pure64_RISCV_SRLI_bv
+  simp
+
+def SHIFTIOP_pure64_RISCV_SRAI (shamt : BitVec 6) (rs1_val : BitVec 64): BitVec 64 :=
+    let value := rs1_val ;
+    let shift := shamt.toNat;
+    BitVec.setWidth 64 (BitVec.extractLsb (63 + shift) shift (BitVec.signExtend (64 + shift) value))
+
+def SHIFTIOP_pure64_RISCV_SRAI_bv (shamt : BitVec 6) (rs1_val : BitVec 64): BitVec 64 :=
+    BitVec.sshiftRight' rs1_val  shamt
+
+theorem SHIFTIOP_pure64_RISCV_SRAI_eq_SHIFTIOP_pure64_RISCV_SRAI_bv
+  (shamt : BitVec 6) (rs1_val : BitVec 64) :
+    SHIFTIOP_pure64_RISCV_SRAI shamt rs1_val =
+    SHIFTIOP_pure64_RISCV_SRAI_bv shamt rs1_val :=
+  by
+  unfold SHIFTIOP_pure64_RISCV_SRAI SHIFTIOP_pure64_RISCV_SRAI_bv
+  simp only [BitVec.sshiftRight_eq']
+  rw [sshiftRight_eq_setWidth_extractLsb_signExtend]
 
 def RTYPEW_pure64_RISCV_ADDW (rs2_val : BitVec 64) (rs1_val : BitVec 64) : BitVec 64 :=
   let rs1_val32 := BitVec.extractLsb' 0 32 rs1_val;
@@ -53,20 +124,67 @@ def RTYPEW_pure64_RISCV_SUBW (rs2_val : BitVec 64) (rs1_val : BitVec 64) : BitVe
   BitVec.signExtend 64 (BitVec.sub rs1_val32 rs2_val32)
 
 def RTYPEW_pure64_RISCV_SLLW (rs2_val : BitVec 64) (rs1_val : BitVec 64) : BitVec 64 :=
-  let rs1_val32 := BitVec.extractLsb' 0 32 rs1_val;
-  let rs2_val32 := BitVec.extractLsb' 0 32 rs2_val;
-  let shamt := BitVec.extractLsb' 0 5 rs2_val32;
-  BitVec.signExtend 64 (rs1_val32 <<< shamt)
+    let rs1_val32 := BitVec.extractLsb' 0 32 rs1_val;
+    let rs2_val32 := BitVec.extractLsb' 0 32 rs2_val;
+    let shamt := BitVec.extractLsb' 0 5 rs2_val32;
+    BitVec.signExtend 64 (BitVec.shiftLeft rs1_val32 shamt.toNat)
+
+def RTYPEW_pure64_RISCV_SLLW_bv (rs2_val : BitVec 64) (rs1_val : BitVec 64) : BitVec 64 :=
+    let rs1_val32 := BitVec.extractLsb' 0 32 rs1_val;
+    let rs2_val32 := BitVec.extractLsb' 0 32 rs2_val;
+    let shamt := BitVec.extractLsb' 0 5 rs2_val32;
+    BitVec.signExtend 64 (rs1_val32 <<< shamt)
+
+theorem RTYPEW_pure64_RISCV_SLLW_eq_RTYPEW_pure64_RISCV_SLLW_bv
+    (rs2_val : BitVec 64) (rs1_val : BitVec 64) :
+    RTYPEW_pure64_RISCV_SLLW rs2_val rs1_val
+    = RTYPEW_pure64_RISCV_SLLW_bv rs2_val rs1_val :=
+  by
+  unfold RTYPEW_pure64_RISCV_SLLW RTYPEW_pure64_RISCV_SLLW_bv
+  simp only [extractLsb'_eq_setWidth, Nat.reduceLeDiff, BitVec.setWidth_setWidth_of_le,
+    BitVec.toNat_setWidth, Nat.reducePow, BitVec.shiftLeft_eq, BitVec.shiftLeft_eq']
 
 def RTYPEW_pure64_RISCV_SRLW (rs2_val : BitVec 64) (rs1_val : BitVec 64) : BitVec 64 :=
-  let rs1_val32 := BitVec.extractLsb' 0 32 rs1_val;
-  let rs2_val32 := BitVec.extractLsb' 0 32 rs2_val;
-  let shamt := BitVec.extractLsb' 0 5 rs2_val32;
-  BitVec.signExtend 64 (rs1_val32 >>> shamt)
+    let rs1_val32 := BitVec.extractLsb' 0 32 rs1_val;
+    let rs2_val32 := BitVec.extractLsb' 0 32 rs2_val;
+    let shamt := BitVec.extractLsb' 0 5 rs2_val32;
+    BitVec.signExtend 64 (BitVec.ushiftRight rs1_val32 shamt.toNat)
 
-def RTYPEW_pure64_RISCV_SRAW (rs2_val : BitVec 64) (rs1_val : BitVec 64) : BitVec 64 :=
-  BitVec.signExtend 64
-  (BitVec.sshiftRight' (BitVec.extractLsb 31 0 rs1_val) (BitVec.extractLsb 4 0 rs2_val))
+def RTYPEW_pure64_RISCV_SRLW_bv (rs2_val : BitVec 64) (rs1_val : BitVec 64) : BitVec 64 :=
+    let rs1_val32 := BitVec.extractLsb' 0 32 rs1_val;
+    let rs2_val32 := BitVec.extractLsb' 0 32 rs2_val;
+    let shamt := BitVec.extractLsb' 0 5 rs2_val32;
+    BitVec.signExtend 64 (rs1_val32 >>> shamt)
+
+theorem RTYPEW_pure64_RISCV_SLLW_eq_RTYPEW_pure64_RISCV_SRLW_bv
+    (rs2_val : BitVec 64) (rs1_val : BitVec 64) :
+    RTYPEW_pure64_RISCV_SRLW rs2_val rs1_val
+    = RTYPEW_pure64_RISCV_SRLW_bv rs2_val rs1_val := by
+  unfold RTYPEW_pure64_RISCV_SRLW RTYPEW_pure64_RISCV_SRLW_bv
+  simp only [extractLsb'_eq_setWidth, Nat.reduceLeDiff, BitVec.setWidth_setWidth_of_le,
+    BitVec.toNat_setWidth, Nat.reducePow, BitVec.ushiftRight_eq, BitVec.ushiftRight_eq']
+
+def RTYPEW_pure64_RISCV_SRAW (rs2_val : BitVec 64) (rs1_val : BitVec 64) :=
+    BitVec.signExtend 64
+           (BitVec.setWidth 32
+              (BitVec.extractLsb
+                 (31 + rs2_val.toNat % 4294967296 % 32)
+                     (rs2_val.toNat % 4294967296 % 32)
+                          (BitVec.signExtend (32 + rs2_val.toNat % 4294967296 % 32)
+                              (BitVec.extractLsb 31 0 rs1_val))))
+
+def RTYPEW_pure64_RISCV_SRAW_bv (rs2_val : BitVec 64) (rs1_val : BitVec 64) :=
+    BitVec.signExtend 64
+    (BitVec.sshiftRight' (BitVec.extractLsb 31 0 rs1_val) (BitVec.extractLsb 4 0 rs2_val))
+
+theorem RTYPEW_pure64_RISCV_SRAW_eq_RTYPEW_pure64_RISCV_SRAW_bv
+    (rs2_val : BitVec 64) (rs1_val : BitVec 64) :
+    RTYPEW_pure64_RISCV_SRAW rs2_val rs1_val
+    = RTYPEW_pure64_RISCV_SRAW_bv rs2_val rs1_val :=
+  by
+  unfold RTYPEW_pure64_RISCV_SRAW RTYPEW_pure64_RISCV_SRAW_bv
+  rw [← sshiftRight_eq_setWidth_extractLsb_signExtend]
+  simp
 
 def RTYPE_pure64_RISCV_ADD (rs2_val : BitVec 64) (rs1_val : BitVec 64) : BitVec 64 :=
   BitVec.add rs1_val rs2_val
@@ -89,171 +207,415 @@ def RTYPE_pure64_RISCV_XOR (rs2_val : BitVec 64) (rs1_val : BitVec 64) : BitVec 
   BitVec.xor rs2_val rs1_val
 
 def RTYPE_pure64_RISCV_SLL (rs2_val : BitVec 64) (rs1_val : BitVec 64) : BitVec 64 :=
-  let shamt := (BitVec.extractLsb 5 0 rs2_val);
-  rs1_val <<< shamt
+    let shamt := (BitVec.extractLsb 5 0 rs2_val).toNat;
+    BitVec.shiftLeft rs1_val shamt
+
+def RTYPE_pure64_RISCV_SLL_bv (rs2_val : BitVec 64) (rs1_val : BitVec 64) : BitVec 64 :=
+    let shamt := (BitVec.extractLsb 5 0 rs2_val);
+    rs1_val <<< shamt
+
+theorem RTYPE_pure64_RISCV_SLL_eq_RTYPE_pure64_RISCV_SLL_bv
+  (rs2_val : BitVec 64) (rs1_val : BitVec 64) :
+    RTYPE_pure64_RISCV_SLL rs2_val rs1_val =
+    RTYPE_pure64_RISCV_SLL_bv rs2_val rs1_val := by
+  unfold RTYPE_pure64_RISCV_SLL  RTYPE_pure64_RISCV_SLL_bv
+  simp
 
 def RTYPE_pure64_RISCV_SRL (rs2_val : BitVec 64) (rs1_val : BitVec 64) : BitVec 64 :=
-  let shamt := (BitVec.extractLsb 5 0 rs2_val)
-  rs1_val  >>> shamt
+  let shamt := (BitVec.extractLsb 5 0 rs2_val).toNat;
+  BitVec.ushiftRight rs1_val shamt
+
+def RTYPE_pure64_RISCV_SRL_bv (rs2_val : BitVec 64) (rs1_val : BitVec 64) : BitVec 64 :=
+  let shamt := BitVec.extractLsb 5 0 rs2_val
+  rs1_val >>> shamt
+
+theorem RTYPE_pure64_RISCV_SRL_eq_RTYPE_pure64_RISCV_SRL_bv
+  (rs2_val : BitVec 64) (rs1_val : BitVec 64) :
+    RTYPE_pure64_RISCV_SRL rs2_val rs1_val =
+    RTYPE_pure64_RISCV_SRL_bv rs2_val rs1_val :=
+  by
+  unfold RTYPE_pure64_RISCV_SRL RTYPE_pure64_RISCV_SRL_bv
+  simp
 
 def RTYPE_pure64_RISCV_SUB (rs2_val : BitVec 64) (rs1_val : BitVec 64) : BitVec 64 :=
   BitVec.sub rs1_val rs2_val
 
-def RTYPE_pure64_RISCV_SRA (rs2_val : BitVec 64) (rs1_val : BitVec 64) : BitVec 64 :=
-  BitVec.sshiftRight' rs1_val  (BitVec.extractLsb 5 0 rs2_val)
+def RTYPE_pure64_RISCV_SRA (rs2_val : BitVec 64) (rs1_val : BitVec 64) :=
+    BitVec.setWidth 64
+      (BitVec.extractLsb
+        (63 + (BitVec.extractLsb 5 0 rs2_val).toNat)
+        (BitVec.extractLsb 5 0 rs2_val).toNat
+        (BitVec.signExtend
+          (64 + (BitVec.extractLsb 5 0 rs2_val).toNat) rs1_val))
+
+def RTYPE_pure64_RISCV_SRA_bv (rs2_val : BitVec 64) (rs1_val : BitVec 64) : BitVec 64 :=
+    BitVec.sshiftRight' rs1_val (BitVec.extractLsb 5 0 rs2_val)
+
+theorem RTYPE_pure64_RISCV_SRA_eqRTYPE_pure64_RISCV_SRA_bv
+  (rs2_val : BitVec 64) (rs1_val : BitVec 64) :
+    RTYPE_pure64_RISCV_SRA  rs2_val rs1_val =
+    RTYPE_pure64_RISCV_SRA_bv rs2_val rs1_val := by
+  unfold RTYPE_pure64_RISCV_SRA RTYPE_pure64_RISCV_SRA_bv
+  rw [BitVec.sshiftRight', sshiftRight_eq_setWidth_extractLsb_signExtend]
 
 /- wip : working on removing toNats and toInts in this definiton, therefore waiting for a
  bit vec lemma to be upstreamed. -/
-def REMW_pure64_unsigned (rs2_val : BitVec 64) (rs1_val : BitVec 64) : BitVec 64 :=
- BitVec.signExtend 64
-    (BitVec.extractLsb' 0 32
-      (BitVec.ofInt 33
-        (if (rs2_val.toNat: Int) % ↑(2 ^ 32) = 0 then (rs1_val.toNat : Int) % ↑(2 ^ 32)
-        else ((rs1_val.toNat: Int) % ↑(2 ^ 32)).tmod ((rs2_val.toNat : Int) % ↑(2 ^ 32)))))
+def REMW_pure64_unsigned (rs2_val : BitVec 64) (rs1_val : BitVec 64): BitVec 64 :=
+    BitVec.signExtend 64
+      (BitVec.extractLsb' 0 32
+        (BitVec.ofInt 33
+          (if ((BitVec.extractLsb 31 0 rs2_val).toNat : Int) = 0 then ↑(BitVec.extractLsb 31 0 rs1_val).toNat
+          else ((BitVec.extractLsb 31 0 rs1_val).toNat : Int).tmod ↑(BitVec.extractLsb 31 0 rs2_val).toNat)))
+
+def REMW_pure64_unsigned_bv (rs2_val : BitVec 64) (rs1_val : BitVec 64) : BitVec 64 :=
+    BitVec.signExtend 64
+      ((BitVec.extractLsb 31 0 rs1_val).umod (BitVec.extractLsb 31 0 rs2_val))
+
+theorem REMW_pure64_unsigned_eq_REMW_pure64_unsigned_bv (rs2_val : BitVec 64) (rs1_val : BitVec 64) :
+    REMW_pure64_unsigned rs2_val rs1_val
+    = REMW_pure64_unsigned_bv rs2_val rs1_val :=
+  by
+  unfold  REMW_pure64_unsigned REMW_pure64_unsigned_bv
+  rw [extractLsb'_ofInt_eq_ofInt (h:= by simp)]
+  split
+  case isTrue ht =>
+      congr
+      rw [BitVec.extractLsb,BitVec.extractLsb]
+      simp only [Nat.sub_zero, Nat.reduceAdd]
+      rw [BitVec.extractLsb] at ht
+      simp only [extractLsb'_eq_setWidth]
+      simp only [Nat.sub_zero, Nat.reduceAdd] at ht
+      norm_cast at ht
+      obtain h : (BitVec.extractLsb' 0 32 rs2_val) = 0#_ :=
+        BitVec.eq_of_toNat_eq ht
+      obtain h1 : (0#32).toNat = 0 := by bv_decide
+      simp only [BitVec.toNat_setWidth, Int.natCast_emod, Int.natCast_pow, Nat.cast_ofNat,
+        BitVec.umod_eq]
+      rw [show 0 = (0#32).toNat by omega, ← BitVec.toNat_eq] at ht
+      conv at ht =>
+        lhs
+        rw [show (0#32).toNat = 0 by omega]
+      rw [← BitVec.setWidth_eq_extractLsb' (by simp)] at ht
+      rw [ht, BitVec.umod_zero, ← BitVec.toInt_inj]
+      simp only [Int.reducePow, BitVec.toInt_ofInt, Nat.reducePow, BitVec.toInt_setWidth]
+      have helper : ((4294967296 : Nat) : Int) = (4294967296 : Int) := rfl
+      rw [← helper, Int.emod_bmod (x := (rs1_val.toNat : Int)) (n := (4294967296))]
+  case isFalse hf =>
+      congr
+      simp only [Nat.sub_zero, Nat.reduceAdd, BitVec.extractLsb_toNat, Nat.shiftRight_zero,
+        Nat.reducePow, Int.natCast_emod, Nat.cast_ofNat, BitVec.umod_eq]
+      simp at hf
+      apply BitVec.eq_of_toInt_eq
+      simp only [BitVec.toInt_ofInt, Nat.reducePow, BitVec.toInt_umod, BitVec.extractLsb_toNat,
+        Nat.shiftRight_zero, Nat.sub_zero, Nat.reduceAdd, Int.natCast_emod, Nat.cast_ofNat]
+      rfl
 
 def REMW_pure64_signed (rs2_val : BitVec 64) (rs1_val : BitVec 64) : BitVec 64 :=
-  BitVec.signExtend 64
-    (BitVec.extractLsb' 0 32
-      (BitVec.ofInt (33)
-        (if (BitVec.extractLsb 31 0 rs2_val).toInt = 0 then (BitVec.extractLsb 31 0 rs1_val).toInt
-        else (BitVec.extractLsb 31 0 rs1_val).toInt.tmod (BitVec.extractLsb 31 0 rs2_val).toInt)))
+    BitVec.signExtend 64
+      (BitVec.extractLsb' 0 32
+        (BitVec.ofInt (33)
+          (if (BitVec.extractLsb 31 0 rs2_val).toInt = 0 then (BitVec.extractLsb 31 0 rs1_val).toInt
+          else (BitVec.extractLsb 31 0 rs1_val).toInt.tmod (BitVec.extractLsb 31 0 rs2_val).toInt)))
+
+def REMW_pure64_signed_bv (rs2_val : BitVec 64) (rs1_val : BitVec 64) : BitVec 64 :=
+    BitVec.signExtend 64
+        ((BitVec.extractLsb 31 0 rs1_val).srem (BitVec.extractLsb 31 0 rs2_val))
+
+theorem REMW_pure64_signed_eq_REMW_pure64_signed (rs2_val : BitVec 64) (rs1_val : BitVec 64) :
+    REMW_pure64_signed rs2_val rs1_val = REMW_pure64_signed_bv rs2_val rs1_val :=
+  by
+  unfold REMW_pure64_signed REMW_pure64_signed_bv
+  rw [extractLsb'_ofInt_eq_ofInt (h:= by simp)]
+  congr
+  split
+  case e_x.isTrue ht  =>
+    obtain h': (BitVec.extractLsb 31 0 rs2_val) = 0#_ :=
+      BitVec.eq_of_toInt_eq ht
+    simp only [Nat.sub_zero, Nat.reduceAdd] at h'
+    simp only [h']
+    rw [BitVec.ofInt_toInt]
+    simp only [Nat.sub_zero, Nat.reduceAdd, BitVec.srem_zero]
+  case e_x.isFalse hf =>
+    rw [← BitVec.toInt_srem, BitVec.ofInt_toInt]
 
 def REM_pure64_unsigned (rs2_val : BitVec 64) (rs1_val : BitVec 64) : BitVec 64 :=
-  BitVec.extractLsb' 0 64
-  (BitVec.ofInt 65 (if (rs2_val.toNat: Int) = 0 then (rs1_val.toNat: Int)  else (rs1_val.toNat :Int).tmod (rs2_val.toNat : Int)))
+     BitVec.extractLsb' 0 64
+      (BitVec.ofInt 65 (if (rs2_val.toNat: Int) = 0 then (rs1_val.toNat: Int)  else (rs1_val.toNat :Int).tmod (rs2_val.toNat : Int)))
+
+def REM_pure64_unsigned_bv (rs2_val : BitVec 64) (rs1_val : BitVec 64) : BitVec 64 :=
+     if rs2_val = 0 then rs1_val else ((rs1_val).umod (rs2_val))
+
+theorem  REM_pure64_unsigned_eq_REM_pure64_unsigned_bv (rs2_val : BitVec 64) (rs1_val : BitVec 64) :
+    REM_pure64_unsigned rs2_val rs1_val = REM_pure64_unsigned_bv rs2_val rs1_val := by
+  unfold REM_pure64_unsigned REM_pure64_unsigned_bv
+  rw [extractLsb'_ofInt_eq_ofInt (h:= by simp )]
+  split
+  case isTrue isZero =>
+      simp only [Int.natCast_eq_zero] at isZero
+      obtain rfl : rs2_val = 0#_ :=
+        BitVec.eq_of_toNat_eq isZero
+      simp
+  case isFalse nonZero =>
+      simp only [Int.natCast_eq_zero] at nonZero
+      simp only [BitVec.ofNat_eq_ofNat, BitVec.umod_eq]
+      have h:= (BitVec.toNat_ne_iff_ne (x:=rs2_val) (y:= 0)).mp nonZero
+      have h2:= (BitVec.toNat_ne_iff_ne (x:=rs2_val) (y:= 0)).mpr h
+      split
+      case isTrue => contradiction
+      case isFalse =>
+        apply BitVec.eq_of_toInt_eq
+        simp only [BitVec.toInt_ofInt, Nat.reducePow, BitVec.toInt_umod]
+        rfl
 
 def REM_pure64_signed (rs2_val : BitVec 64) (rs1_val : BitVec 64) : BitVec 64 :=
-  BitVec.extractLsb' 0 64
-  (BitVec.ofInt 65 (if rs2_val.toInt = 0 then rs1_val.toInt else rs1_val.toInt.tmod rs2_val.toInt))
+    BitVec.extractLsb' 0 64
+    (BitVec.ofInt 65 (if rs2_val.toInt = 0 then rs1_val.toInt else rs1_val.toInt.tmod rs2_val.toInt))
 
--- wip: getting rid of toInt and toNat
-def MULW_pure64 (rs2_val : (BitVec 64)) (rs1_val : BitVec 64) : BitVec 64 :=
-  BitVec.signExtend 64
-    (BitVec.extractLsb 31 0
-      (BitVec.extractLsb' 0 64
-        (BitVec.ofInt 65 ((BitVec.extractLsb 31 0 rs1_val).toInt * (BitVec.extractLsb 31 0 rs2_val).toInt))))
+def REM_pure64_signed_bv (rs2_val : BitVec 64) (rs1_val : BitVec 64) : BitVec 64 :=
+    rs1_val.srem rs2_val
+
+theorem REM_pure64_signed_eq_REM_pure64_signed_bv (rs2_val : BitVec 64) (rs1_val : BitVec 64) :
+    REM_pure64_signed rs2_val rs1_val = REM_pure64_signed_bv rs2_val rs1_val := by
+  unfold REM_pure64_signed REM_pure64_signed_bv
+  rw [extractLsb'_ofInt_eq_ofInt (h:= by simp)]
+  split
+  case isTrue ht  =>
+    simp only [BitVec.ofInt_toInt, BitVec.srem, BitVec.umod_eq, BitVec.neg_eq]
+    obtain rfl : rs2_val = 0#_ :=
+      BitVec.eq_of_toInt_eq ht
+    split <;> simp
+  case isFalse hf =>
+    rw [← BitVec.toInt_srem, BitVec.ofInt_toInt]
+
+def MULW_pure64 (rs2_val : BitVec 64) (rs1_val : BitVec 64) : BitVec 64 :=
+    BitVec.signExtend 64
+      (BitVec.extractLsb 31 0
+        (BitVec.extractLsb' 0 64
+          (BitVec.ofInt 65 ((BitVec.extractLsb 31 0 rs1_val).toInt * (BitVec.extractLsb 31 0 rs2_val).toInt))))
+
+def MULW_pure64_bv (rs2_val : BitVec 64) (rs1_val : BitVec 64) : BitVec 64 :=
+    BitVec.signExtend 64
+      (((BitVec.extractLsb 31 0 rs1_val) * (BitVec.extractLsb 31 0 rs2_val)))
+
+theorem MULW_pure64_eq_MULW_pure64_bv (rs2_val : BitVec 64) (rs1_val : BitVec 64) :
+    MULW_pure64 rs2_val rs1_val = MULW_pure64_bv rs2_val rs1_val :=
+  by
+  unfold MULW_pure64 MULW_pure64_bv
+  rw [extractLsb'_ofInt_eq_ofInt (h:= by simp), BitVec.extractLsb]
+  simp only [Nat.sub_zero, Nat.reduceAdd]
+  rw [extractLsb'_ofInt_eq_ofInt (h:= by simp)]
+  congr
+  apply BitVec.eq_of_toInt_eq
+  simp only [BitVec.toInt_extractLsb, Nat.shiftRight_zero, Nat.sub_zero, Nat.reduceAdd,
+    Nat.reducePow, BitVec.toInt_ofInt, Int.mul_bmod_bmod, Int.bmod_mul_bmod, BitVec.toInt_mul]
+
 /-!
 ## mul operations flags
  the suffix indicates how the flags are assumed to be set.
 { high := _, signed_rs1:= _, signed_rs2 := _  }
 -/
 def MUL_pure64_fff (rs2_val : BitVec 64) (rs1_val : BitVec 64) : BitVec 64 :=
-  rs2_val * rs1_val
+     BitVec.extractLsb 63 0 (BitVec.extractLsb' 0 128 (BitVec.ofInt 129 (rs1_val.toNat * rs2_val.toNat)))
+
+def MUL_pure64_fff_bv (rs2_val : BitVec 64) (rs1_val : BitVec 64) : BitVec 64 :=  rs2_val * rs1_val
+
+theorem MUL_pure64_fff_eq_MUL_pure64_fff_bv (rs2_val : BitVec 64) (rs1_val : BitVec 64) :
+    MUL_pure64_fff  rs2_val rs1_val = MUL_pure64_fff_bv rs2_val rs1_val := by
+  simp only  [MUL_pure64_fff,  MUL_pure64_fff_bv]
+  apply BitVec.eq_of_toNat_eq
+  simp [Nat.sub_zero, Nat.reduceAdd, Int.mul_def, BitVec.extractLsb_toNat,
+    BitVec.extractLsb'_toNat, BitVec.toNat_ofInt, Nat.reducePow, Nat.cast_ofNat,
+    Nat.shiftRight_zero, Nat.reduceDvd, Nat.mod_mod_of_dvd, BitVec.mul_eq, BitVec.toNat_mul]
+  congr
+  norm_cast
+  rw [Int.toNat_natCast, Nat.mod_eq_of_lt]
+  ac_rfl
+  have aa := BitVec.isLt rs1_val
+  have bb := BitVec.isLt rs2_val
+  have := @Nat.mul_lt_mul'' _ _ _ _ aa bb
+  simp only [Nat.reducePow, Nat.reduceMul] at this
+  omega
 
 def  MUL_pure64_fft (rs2_val : BitVec 64) (rs1_val : BitVec 64) : BitVec 64 :=
   BitVec.extractLsb 63 0
     (BitVec.extractLsb' 0 128
       (BitVec.ofInt 129 (Int.ofNat (Int.mul (Int.ofNat rs1_val.toNat)  (rs2_val.toInt)).toNat)))
---wip
-def MUL_pure64_ftf (rs2_val : BitVec 64) (rs1_val : BitVec 64)  : BitVec 64 :=
+
+def MUL_pure64_ftf (rs2_val : BitVec 64) (rs1_val : BitVec 64) : BitVec 64 :=
   BitVec.extractLsb 63 0 (BitVec.extractLsb' 0 128 (BitVec.ofInt 129 (rs1_val.toInt * rs2_val.toNat)))
 
---wip
 def MUL_pure64_tff (rs2_val : BitVec 64) (rs1_val : BitVec 64) : BitVec 64 :=
-  BitVec.extractLsb 127 64 (BitVec.extractLsb' 0 128 (BitVec.ofInt 129 (rs1_val.toNat * rs2_val.toNat)))
+    BitVec.extractLsb 127 64 (BitVec.extractLsb' 0 128 (BitVec.ofInt 129 (rs1_val.toNat * rs2_val.toNat)))
 
--- wip
-def MUL_pure64_tft (rs2_val : BitVec 64) (rs1_val : BitVec 64) : BitVec 64 :=
-   BitVec.extractLsb 127 64 (BitVec.extractLsb' 0 128 (BitVec.ofInt 129 (rs1_val.toNat * rs2_val.toInt)))
+def MUL_pure64_tff_bv  (rs2_val : BitVec 64) (rs1_val : BitVec 64) : BitVec 64 :=
+   BitVec.extractLsb 127 64 (BitVec.extractLsb' 0 128 ((BitVec.zeroExtend 128 rs1_val)  * (BitVec.zeroExtend 128 rs2_val)))
 
--- wip
+theorem MUL_pure64_tff_eq_MUL_pure64_tff_bv (rs2_val : BitVec 64) (rs1_val : BitVec 64) :
+    MUL_pure64_tff rs2_val rs1_val = MUL_pure64_tff_bv rs2_val rs1_val := by
+  unfold  MUL_pure64_tff MUL_pure64_tff_bv
+  suffices (BitVec.extractLsb' 0 128 (BitVec.ofInt 129 (↑rs1_val.toNat * ↑rs2_val.toNat))) =
+                 (BitVec.extractLsb' 0 128 (BitVec.zeroExtend 128 rs1_val * BitVec.zeroExtend 128 rs2_val))
+    by
+    congr
+  apply BitVec.eq_of_toNat_eq
+  simp only [HMul.hMul, Mul.mul]
+  simp only [Int.mul_def, extractLsb'_eq_setWidth, BitVec.toNat_setWidth, BitVec.toNat_ofInt,
+      Nat.reducePow, Nat.cast_ofNat, BitVec.truncate_eq_setWidth, BitVec.mul_eq,
+      BitVec.extractLsb'_eq_self, BitVec.toNat_mul, Nat.mul_mod_mod, Nat.mod_mul_mod]
+  congr
+  norm_cast
+  rw [Int.toNat_natCast]
+  have aa := BitVec.isLt rs1_val
+  have bb := BitVec.isLt rs2_val
+  have cc : 680564733841876926926749214863536422912 = 2^129 := by native_decide
+  have aaa : rs1_val.toNat >= 0 := by simp
+  have bbb : rs2_val.toNat >= 0 := by simp
+  rw [Nat.mod_eq_of_lt (h:=
+      by
+      rw [cc]
+      have := Nat.mul_lt_mul''
+        (a := rs1_val.toNat) (b := rs2_val.toNat) (c := 2 ^ 64) (d := 2 ^ 64) aa bb
+      omega )]
+  have := @Nat.mul_lt_mul'' _ _ _ _ aa bb
+  omega
+
 def MUL_pure64_ttf (rs2_val : BitVec 64) (rs1_val : BitVec 64) : BitVec 64 :=
-  BitVec.extractLsb 127 64 (BitVec.extractLsb' 0 128 (BitVec.ofInt 129 (rs1_val.toInt * rs2_val.toNat)))
+    BitVec.extractLsb 127 64 (BitVec.extractLsb' 0 128 (BitVec.ofInt 129 (rs1_val.toInt * rs2_val.toNat)))
 
+def MUL_pure64_ttf_bv (rs2_val : BitVec 64) (rs1_val : BitVec 64) : BitVec 64 :=
+    BitVec.extractLsb 127 64 (((BitVec.signExtend 129 rs1_val ) * (BitVec.zeroExtend 129 rs2_val )))
+
+theorem MUL_pure64_ttf_eq_MUL_pure64_ttf_bv (rs2_val : BitVec 64) (rs1_val : BitVec 64) :
+    MUL_pure64_ttf rs2_val rs1_val = MUL_pure64_ttf_bv rs2_val rs1_val := by
+  unfold MUL_pure64_ttf MUL_pure64_ttf_bv
+  simp only [extractLsb'_eq_setWidth, BitVec.truncate_eq_setWidth]
+  have h1 : rs1_val.toInt = (rs1_val.signExtend 129).toInt := by
+      simp only [Nat.reduceLeDiff, BitVec.toInt_signExtend_of_le]
+  simp only [h1]
+  have h2 : rs2_val.toNat = (rs2_val.zeroExtend 129).toInt := by
+      simp only [BitVec.truncate_eq_setWidth, BitVec.toInt_setWidth]
+      have : rs2_val.toNat < 2 ^64 := by omega
+      have := Nat.pow_lt_pow_of_lt (a := 2) (n := 64) (m := 129) (by omega) (by omega)
+      rw [Int.bmod_eq_of_le (n := (rs2_val.toNat : Int)) (by omega) (by omega)]
+  rw [h2]
+  simp only [BitVec.truncate_eq_setWidth, BitVec.toInt_setWidth, Nat.reducePow, BitVec.ofInt_mul,
+    BitVec.ofInt_toInt]
+  rw [Int.bmod_eq_of_le (n := (rs2_val.toNat : Int)) (by omega) (by omega)]
+  simp only [BitVec.ofInt_natCast, BitVec.ofNat_toNat]
+  rw [extractLsb_setWidth_of_lt (hi := 127) (lo := 64) (v := 128) (x := BitVec.signExtend 129 rs1_val * BitVec.setWidth 129 rs2_val) (by omega) (by omega)]
 def MUL_pure64_ftt (rs2_val : BitVec 64) (rs1_val : BitVec 64) : BitVec 64 :=
   rs2_val * rs1_val
 
--- wip: need to remove toInts and toNats
 def MUL_pure64_ttt (rs2_val : BitVec 64) (rs1_val : BitVec 64) : BitVec 64 :=
-  BitVec.extractLsb 127 64 (BitVec.extractLsb' 0 128 (BitVec.ofInt 129 (rs1_val.toInt * rs2_val.toInt)))
+    BitVec.extractLsb 127 64 (BitVec.extractLsb' 0 128 (BitVec.ofInt 129 (rs1_val.toInt * rs2_val.toInt)))
+
+def MUL_pure64_ttt_bv  (rs2_val : BitVec 64) (rs1_val : BitVec 64) : BitVec 64 :=
+    BitVec.extractLsb 127 64 ((BitVec.signExtend 129 rs1_val) * (BitVec.signExtend 129 rs2_val))
+
+theorem MUL_pure64_ttt_eq_MUL_pure64_ttt_bv (rs2_val : BitVec 64) (rs1_val : BitVec 64) :
+    MUL_pure64_ttt rs2_val rs1_val = MUL_pure64_ttt_bv rs2_val rs1_val :=
+   by
+    unfold MUL_pure64_ttt_bv MUL_pure64_ttt
+    have : rs1_val.toInt = (rs1_val.signExtend 129).toInt := by
+      simp only [Nat.reduceLeDiff, BitVec.toInt_signExtend_of_le]
+    simp only [this]
+    have : rs2_val.toInt = (rs2_val.signExtend 129).toInt := by
+      simp only [Nat.reduceLeDiff, BitVec.toInt_signExtend_of_le]
+    simp only [this]
+    rw [BitVec.ofInt_mul]
+    simp only [BitVec.ofInt_toInt, extractLsb'_eq_setWidth]
+    rw [extractLsb_setWidth_of_lt (hi := 127) (lo := 64) (v := 128) (x := BitVec.signExtend 129 rs1_val * BitVec.signExtend 129 rs2_val) (by omega)]
+    simp
+
+
 -- wip: need to remove toInts and toNats
 def DIVW_pure64_signed (rs2_val : BitVec 64) (rs1_val : BitVec 64) : BitVec 64 :=
-  BitVec.signExtend 64
-    (BitVec.extractLsb' 0 32
-      (BitVec.ofInt 33
-        (if
-            2147483647 <
-              if (BitVec.extractLsb 31 0 rs2_val).toInt = 0 then -1
-              else (BitVec.extractLsb 31 0 rs1_val).toInt.tdiv (BitVec.extractLsb 31 0 rs2_val).toInt then
-          -2147483648
-        else
-          if (BitVec.extractLsb 31 0 rs2_val).toInt = 0 then -1
-          else (BitVec.extractLsb 31 0 rs1_val).toInt.tdiv (BitVec.extractLsb 31 0 rs2_val).toInt)))
+    BitVec.signExtend 64
+      (BitVec.extractLsb' 0 32
+        (BitVec.ofInt 33
+          (if
+              2147483647 <
+                if (BitVec.extractLsb 31 0 rs2_val).toInt = 0 then -1
+                else (BitVec.extractLsb 31 0 rs1_val).toInt.tdiv (BitVec.extractLsb 31 0 rs2_val).toInt then
+            -2147483648
+          else
+            if (BitVec.extractLsb 31 0 rs2_val).toInt = 0 then -1
+            else (BitVec.extractLsb 31 0 rs1_val).toInt.tdiv (BitVec.extractLsb 31 0 rs2_val).toInt)))
 
 -- wip: need to remove toInts and toNats
 def  DIVW_pure64_unsigned (rs2_val : BitVec 64) (rs1_val : BitVec 64) : BitVec 64 :=
-  BitVec.signExtend 64
-   (BitVec.extractLsb' 0 32
-    (BitVec.ofInt 33
-     (if (rs2_val.toNat: Int)  % 4294967296 = 0 then -1
-      else ((rs1_val.toNat : Int) % 4294967296).tdiv ((rs2_val.toNat : Int) % 4294967296))))
+    BitVec.signExtend 64
+      (BitVec.extractLsb' 0 32
+        (BitVec.ofInt 33
+        (if (rs2_val.toNat: Int)  % 4294967296 = 0 then -1
+          else ((rs1_val.toNat : Int) % 4294967296).tdiv ((rs2_val.toNat : Int) % 4294967296))))
 
 def DIV_pure64_signed (rs2_val : BitVec 64) (rs1_val : BitVec 64) : BitVec 64 :=
-  if rs2_val = 0#64 then
-    -1#64
-  else
-    rs1_val.sdiv rs2_val
+    if rs2_val = 0#64 then
+      -1#64
+    else
+      rs1_val.sdiv rs2_val
 
 def DIV_pure64_unsigned (rs2_val : BitVec 64) (rs1_val : BitVec 64) : BitVec 64 :=
-  if rs2_val = 0#64 then
-    (-1)
-  else
-    rs1_val.udiv rs2_val
+    if rs2_val = 0#64 then
+     (-1)
+    else
+      rs1_val.udiv rs2_val
 
 def ITYPE_pure64_RISCV_ADDI (imm : BitVec 12) (rs1_val : BitVec 64) : BitVec 64 :=
-  let immext : BitVec 64 := (BitVec.signExtend 64 imm) ;
-  BitVec.add rs1_val immext
+    let immext : BitVec 64 := (BitVec.signExtend 64 imm) ;
+    BitVec.add rs1_val immext
 
 def ITYPE_pure64_RISCV_SLTI (imm : BitVec 12) (rs1_val : BitVec 64) : BitVec 64 :=
-  let immext : BitVec 64 := (BitVec.signExtend 64 imm);
-  let b := BitVec.slt rs1_val immext;
-  BitVec.zeroExtend 64 (BitVec.ofBool b)
+    let immext : BitVec 64 := (BitVec.signExtend 64 imm);
+    let b := BitVec.slt rs1_val immext;
+    BitVec.zeroExtend 64 (BitVec.ofBool b)
 
 def ITYPE_pure64_RISCV_SLTIU (imm : BitVec 12) (rs1_val : BitVec 64) : BitVec 64 :=
-  let immext : BitVec 64 := (BitVec.signExtend 64 imm);
-  let b := BitVec.ult rs1_val immext;
-  BitVec.setWidth 64 (BitVec.ofBool b)
+    let immext : BitVec 64 := (BitVec.signExtend 64 imm);
+    let b := BitVec.ult rs1_val immext;
+    BitVec.setWidth 64 (BitVec.ofBool b)
 
 def  ITYPE_pure64_RISCV_ANDI (imm : BitVec 12) (rs1_val : BitVec 64) : BitVec 64 :=
-  let immext : BitVec 64 := (BitVec.signExtend 64 imm);
-  BitVec.and rs1_val immext
+    let immext : BitVec 64 := (BitVec.signExtend 64 imm);
+    BitVec.and rs1_val immext
 
 def ITYPE_pure64_RISCV_ORI (imm : BitVec 12) (rs1_val : BitVec 64) : BitVec 64 :=
-  let immext : BitVec 64 := (BitVec.signExtend 64 imm) ;
-  BitVec.or rs1_val immext
+    let immext : BitVec 64 := (BitVec.signExtend 64 imm) ;
+    BitVec.or rs1_val immext
 
 def  ITYPE_pure64_RISCV_XORI (imm : BitVec 12) (rs1_val : BitVec 64) : BitVec 64 :=
-  let immext : BitVec 64 := (BitVec.signExtend 64 imm) ;
-  BitVec.xor rs1_val immext
+    let immext : BitVec 64 := (BitVec.signExtend 64 imm) ;
+    BitVec.xor rs1_val immext
 
 def ZICOND_RTYPE_pure64_RISCV_CZERO_EQZ (rs2_val : BitVec 64) (rs1_val : BitVec 64) :=
-  if rs2_val = BitVec.zero 64 then BitVec.zero 64 else rs1_val
+    if rs2_val = BitVec.zero 64 then BitVec.zero 64 else rs1_val
 
 def ZICOND_RTYPE_pure64_RISCV_RISCV_CZERO_NEZ (rs2_val : BitVec 64) (rs1_val : BitVec 64) :=
-   if rs2_val = BitVec.zero 64 then rs1_val else BitVec.zero 64
+    if rs2_val = BitVec.zero 64 then rs1_val else BitVec.zero 64
 
 def ZBS_RTYPE_pure64_RISCV_BCLR (rs2_val : BitVec 64) (rs1_val : BitVec 64) : BitVec 64 :=
-  BitVec.and rs1_val (BitVec.not ((BitVec.zeroExtend 64 1#1) <<< (BitVec.extractLsb  5 0 rs2_val)))
+    BitVec.and rs1_val (BitVec.not ((BitVec.zeroExtend 64 1#1) <<< (BitVec.extractLsb  5 0 rs2_val)))
 
 def ZBB_EXTOP_pure64_RISCV_SEXTB (rs1_val : BitVec 64) : BitVec 64 :=
-  BitVec.signExtend 64 (BitVec.extractLsb 7 0 rs1_val)
+    BitVec.signExtend 64 (BitVec.extractLsb 7 0 rs1_val)
 
 def ZBB_EXTOP_pure64_RISCV_SEXTH (rs1_val : BitVec 64) : BitVec 64 :=
-  BitVec.signExtend 64 (BitVec.extractLsb 15 0 rs1_val)
+    BitVec.signExtend 64 (BitVec.extractLsb 15 0 rs1_val)
 
 def ZBB_EXTOP_pure64_RISCV_ZEXTH (rs1_val : BitVec 64) : BitVec 64 :=
-  BitVec.zeroExtend 64 (BitVec.extractLsb 15 0 rs1_val)
+    BitVec.zeroExtend 64 (BitVec.extractLsb 15 0 rs1_val)
 
 def ZBS_RTYPE_pure64_RISCV_BEXT (rs2_val : BitVec 64) (rs1_val : BitVec 64) : BitVec 64  :=
-  BitVec.setWidth 64
-    (match
-      BitVec.and rs1_val ((BitVec.setWidth 64 1#1) <<< (BitVec.extractLsb 5 0 rs2_val)) !=
-        0#64 with
-    | true => 1#1
-    | false => 0#1)
+    BitVec.setWidth 64
+      (match
+        BitVec.and rs1_val ((BitVec.setWidth 64 1#1) <<< (BitVec.extractLsb 5 0 rs2_val)) !=
+          0#64 with
+      | true => 1#1
+      | false => 0#1)
 
  def ZBS_RTYPE_pure64_BINV (rs2_val : BitVec 64) (rs1_val : BitVec 64) : BitVec 64 :=
-  BitVec.xor rs1_val ((BitVec.zeroExtend 64 1#1) <<< (BitVec.extractLsb 5 0 rs2_val))
+    BitVec.xor rs1_val ((BitVec.zeroExtend 64 1#1) <<< (BitVec.extractLsb 5 0 rs2_val))
 
 def ZBS_RTYPE_pure64_RISCV_BSET (rs2_val : BitVec 64) (rs1_val : BitVec 64) :=
     BitVec.or rs1_val ((BitVec.zeroExtend 64 1#1) <<< (BitVec.extractLsb 5 0 rs2_val))
@@ -262,7 +624,7 @@ def ZBS_IOP_pure64_RISCV_BCLRI (shamt : BitVec 6) (rs1_val : BitVec 64) : BitVec
     BitVec.and rs1_val (BitVec.not ((BitVec.setWidth 64 1#1) <<< shamt))
 
 def ZBS_IOP_pure64_RISCV_BEXTI (shamt : BitVec 6) (rs1_val : BitVec 64) : BitVec 64 :=
-  BitVec.setWidth 64
+    BitVec.setWidth 64
       (match (BitVec.and (rs1_val) ((BitVec.setWidth 64 1#1) <<< shamt)) != 0#64 with
       | true => 1#1
       | false => 0#1)
@@ -271,53 +633,53 @@ def ZBS_IOP_pure64_RISCV_BINVI (shamt : BitVec 6) (rs1_val : BitVec 64) : BitVec
     BitVec.xor rs1_val  ((BitVec.zeroExtend 64 1#1) <<< shamt)
 
 def ZBS_IOP_pure64_RISCV_BSETI (shamt : BitVec 6) (rs1_val : BitVec 64) : BitVec 64 :=
-  BitVec.or rs1_val ((BitVec.zeroExtend 64 1#1) <<< shamt)
+    BitVec.or rs1_val ((BitVec.zeroExtend 64 1#1) <<< shamt)
 
 -- wip: remove toNats
 def ZBB_RTYPEW_pure64_RISCV_RORW (rs2_val : BitVec 64) (rs1_val : BitVec 64) : BitVec 64 :=
-  BitVec.signExtend (64)
-      (BitVec.or (BitVec.ushiftRight (BitVec.setWidth 32 rs1_val) (rs2_val.toNat % 32))
-        (BitVec.shiftLeft (BitVec.setWidth 32 rs1_val)
-          ((2 ^ 5 - rs2_val.toNat % 32 +
-              32 % 2 ^ (5 + 1)) %
-            2 ^ 5)))
+    BitVec.signExtend (64)
+        (BitVec.or (BitVec.ushiftRight (BitVec.setWidth 32 rs1_val) (rs2_val.toNat % 32))
+          (BitVec.shiftLeft (BitVec.setWidth 32 rs1_val)
+            ((2 ^ 5 - rs2_val.toNat % 32 +
+                32 % 2 ^ (5 + 1)) %
+              2 ^ 5)))
 
 -- wip: remove toNats
 def ZBB_RTYPEW_pure64_RISCV_ROLW (rs2_val : BitVec 64) (rs1_val : BitVec 64) : BitVec 64 :=
-  BitVec.signExtend 64
-    (BitVec.or (BitVec.shiftLeft (BitVec.setWidth 32 rs1_val) (BitVec.extractLsb 4 0 rs2_val).toNat)
-      (BitVec.ushiftRight (BitVec.setWidth 32 rs1_val)
-        (((BitVec.sub ((BitVec.extractLsb' 0 5
-            (BitVec.ofInt 6 32)))
-          (BitVec.extractLsb 4 0 rs2_val)))).toNat))
+    BitVec.signExtend 64
+      (BitVec.or (BitVec.shiftLeft (BitVec.setWidth 32 rs1_val) (BitVec.extractLsb 4 0 rs2_val).toNat)
+        (BitVec.ushiftRight (BitVec.setWidth 32 rs1_val)
+          (((BitVec.sub ((BitVec.extractLsb' 0 5
+              (BitVec.ofInt 6 32)))
+            (BitVec.extractLsb 4 0 rs2_val)))).toNat))
 
  def ZBB_RTYPE_pure64_RISCV_ROL (rs2_val : BitVec 64) (rs1_val : BitVec 64) : BitVec 64 :=
-  BitVec.or (BitVec.shiftLeft  rs1_val (BitVec.extractLsb 5 0 rs2_val).toNat)
-    (rs1_val >>> (BitVec.extractLsb' 0 6 (64#7) - BitVec.extractLsb 5 0 rs2_val))
+    BitVec.or (BitVec.shiftLeft  rs1_val (BitVec.extractLsb 5 0 rs2_val).toNat)
+      (rs1_val >>> (BitVec.extractLsb' 0 6 (64#7) - BitVec.extractLsb 5 0 rs2_val))
 
  def ZBB_RTYPE_pure64_RISCV_ROR (rs2_val : BitVec 64) (rs1_val : BitVec 64) : BitVec 64 :=
-  BitVec.or (rs1_val >>> (BitVec.extractLsb 5 0 rs2_val))
-    (rs1_val <<< ((BitVec.extractLsb' 0 6 (BitVec.ofInt (7) (64)) - BitVec.extractLsb 5 0 rs2_val)))
+    BitVec.or (rs1_val >>> (BitVec.extractLsb 5 0 rs2_val))
+      (rs1_val <<< ((BitVec.extractLsb' 0 6 (BitVec.ofInt (7) (64)) - BitVec.extractLsb 5 0 rs2_val)))
 
  def ZBA_RTYPEUW_pure64_RISCV_ADDUW (rs2_val : BitVec 64) (rs1_val : BitVec 64) : BitVec 64 :=
-  BitVec.zeroExtend 64 (BitVec.extractLsb 31 0 rs1_val) <<< 0#2 + rs2_val
+    BitVec.zeroExtend 64 (BitVec.extractLsb 31 0 rs1_val) <<< 0#2 + rs2_val
 
 def ZBA_RTYPEUW_pure64_RISCV_SH1ADDUW (rs2_val : BitVec 64) (rs1_val : BitVec 64) : BitVec 64 :=
-  BitVec.add (BitVec.zeroExtend 64 (BitVec.extractLsb 31 0 rs1_val) <<< 1#2)  rs2_val
+    BitVec.add (BitVec.zeroExtend 64 (BitVec.extractLsb 31 0 rs1_val) <<< 1#2)  rs2_val
 
 def ZBA_RTYPEUW_pure64_RISCV_SH2ADDUW (rs2_val : BitVec 64) (rs1_val : BitVec 64) : BitVec 64 :=
-  BitVec.add (BitVec.zeroExtend 64 (BitVec.extractLsb 31 0 rs1_val) <<< 2#2) rs2_val
+    BitVec.add (BitVec.zeroExtend 64 (BitVec.extractLsb 31 0 rs1_val) <<< 2#2) rs2_val
 
 def  ZBA_RTYPEUW_pure64_RISCV_SH3ADDUW (rs2_val : BitVec 64) (rs1_val : BitVec 64) : BitVec 64 :=
-  BitVec.add (BitVec.zeroExtend 64 (BitVec.extractLsb 31 0 rs1_val) <<< 3#2)  rs2_val
+    BitVec.add (BitVec.zeroExtend 64 (BitVec.extractLsb 31 0 rs1_val) <<< 3#2)  rs2_val
 
 def ZBA_RTYPE_pure64_RISCV_SH1ADD (rs2_val : BitVec 64) (rs1_val : BitVec 64) : BitVec 64 :=
-  BitVec.add (rs1_val <<< 1#2) rs2_val
+    BitVec.add (rs1_val <<< 1#2) rs2_val
 
 def ZBA_RTYPE_pure64_RISCV_SH2ADD (rs2_val : BitVec 64) (rs1_val : BitVec 64) : BitVec 64 :=
-  BitVec.add (rs1_val <<< 2#2) rs2_val
+    BitVec.add (rs1_val <<< 2#2) rs2_val
 
 def ZBA_RTYPE_pure64_RISCV_SH3ADD(rs2_val : BitVec 64) (rs1_val : BitVec 64) : BitVec 64 :=
-  BitVec.add (rs1_val <<< 3#2) rs2_val
+    BitVec.add (rs1_val <<< 3#2) rs2_val
 
 end RV64Semantics
